%\documentclass[11pt]{article}
\documentclass[a4paper]{article}

%\setlength{\textwidth}{210mm}\setlength{\textheight}{297mm}

\usepackage[utf8]{inputenc}
\usepackage[margin=1.25cm]{geometry}
\usepackage{amsmath}

\usepackage[slovene]{babel}
\usepackage{amssymb}
\usepackage{latexsym}
\usepackage{amsfonts}
\usepackage{amsmath}
\usepackage{arydshln}
\usepackage{amscd}
\usepackage{times}
\usepackage{graphics}
\usepackage{graphicx}
%\usepackage{subfigure}
\usepackage{comment}
\usepackage{float}
% \usepackage{concmath}
\usepackage[T1]{fontenc}
\usepackage{cite}
\usepackage{url}
\usepackage{hyperref}
\usepackage{color}
\usepackage[version=3]{mhchem}
\usepackage{wrapfig}
\usepackage{mathtools}
\usepackage{color}
\usepackage{caption}
\usepackage{subcaption}
\usepackage{makeidx}
\usepackage{tikz}
\usepackage[nodayofweek,level]{datetime}
\usepackage{concrete}

\renewcommand{\vec}[1]{\mathbf{#1}}

\setlength{\parindent}{0pt}
\setlength{\parskip}{0.5ex}

\newtheorem{theorem}{Theorem}
\newtheorem{definition}[theorem]{Definition}
\newtheorem{notation}[theorem]{Notation}

\newtheorem{example}[theorem]{Example}
\newtheorem{proposition}[theorem]{Proposition}
\newtheorem{claim}[theorem]{Claim}
\newtheorem{terminology}[theorem]{Terminology}

\begin{comment}
\newtheorem{comment}[theorem]{Comment}
\end{comment}

\setcounter{secnumdepth}{2}

\begin{document}

\title{Title}

\author{jerneju@gmail.com}

\date{\today}



\maketitle

\section{What to do?}
	\begin{equation}
		J(\theta) = \frac{1}{m}\sum_{i=1}^m \big[-y^{i} \log (h_{\theta} (x^{(i)}))
		- (1 - y^{(i)}) \log(1 - h_{\theta}(x^{(i)}))\big]
		+ \frac{\lambda}{2 m} \sum_{j=1}^n \theta_j^2
	\end{equation}
	\begin{equation}
		\frac{\partial J(\theta)}{\partial \theta_0} = \frac{1}{m} \sum_{i=1}^m
		\big(h_{\theta}(x^{(i)}) - y^{i}\big) x_j^{(i)}
	\end{equation}
	\begin{equation}
		\frac{\partial J(\theta)}{\partial \theta_j} = \bigg(\frac{1}{m} \sum_{i=1}^m
		\big(h_{\theta}(x^{(i)}) - y^{i}\big) x_j^{(i)}\bigg) + \frac{\lambda}{m} \theta_j
	\end{equation}
	\begin{equation}
		J(\theta) = \frac{1}{m}\sum_{i=1}^m \sum_{k=1}^K \bigg[-y_k^{(i)} 
		\log ((h_{\theta}(x^{(i)}))_k) - (1 - y_k^{(i)}) 
		\log (1 - (h_{\theta}(x^{(i)}))_k)\bigg]
	\end{equation}
	\begin{equation}
		\frac{\lambda}{2 m} \bigg[\sum_{j=1}^{25} \sum_{k=1}^{400}\bigg]
	\end{equation}



\end{document}